CollFree behind DecEq, simultaneous games, simultaneous games equiv to turn-based (half) and big protocol?

FraudProof/Games/Base/Simultaneous.lean
@@ -37,7 +37,7 @@ def simultaneous_game {α ℍ : Type}
   --
   : SimWinner
   := match public_data, lplayer , rplayer with
-     | .leaf p , .leaf lp , .leaf _rp =>
+     | .leaf p , .leaf lp , _ =>
        match lp with
          | .none => .Right
          | .some llp =>
@@ -53,9 +53,11 @@ def simultaneous_game {α ℍ : Type}
            (simultaneous_game gr lr lp.2 rr)
      -------
      | .leaf _ , .node _ _ _, _ => .Right
-     | .leaf _ ,  _ , .node _ _ _ => .Left
+     -- | .leaf _ , .leaf .none , _ => .Right
+     -- | .leaf _ , .leaf (.some _) , .node _ _ _ => .Left
      | .node _ _ _, .leaf _ , _ => .Right
-     | .node _ _ _,  _ , .leaf _ => .Left
+     | .node _ _ _, .node (.some _) _ _ , .leaf _ => .Left
+     | .node _ _ _, .node .none _ _ , .leaf  _ => .Right
 
 def gen_to_chooser {ℍ : Type}[DecidableEq ℍ]
   (md : Option (ℍ × ℍ)) (a : ℍ × ℍ × ℍ) : Option ChooserMoves
@@ -79,12 +81,142 @@ theorem eq_sim_games {α ℍ : Type}
          (rplayer.map id gen_to_chooser) = Player.Proposer
     ↔
     simultaneous_game pub lplayer lplayer_commit rplayer = .Left )
-    ∧
-    (treeArbitrationGame ⟨ pub.toB , lplayer_commit⟩ lplayer
-        (rplayer.map id gen_to_chooser) = Player.Chooser
-        ↔
-    simultaneous_game pub lplayer lplayer_commit rplayer = .Right)
-    := sorry
+    -- ∧
+    -- (treeArbitrationGame ⟨ pub.toB , lplayer_commit⟩ lplayer
+    --     (rplayer.map id gen_to_chooser) = Player.Chooser
+    --     ↔
+    -- simultaneous_game pub lplayer lplayer_commit rplayer = .Right)
+    := by
+    apply Iff.intro
+    -- Tree imples simultaneous
+    · revert rplayer lplayer_commit lplayer
+      induction pub with
+      | leaf v =>
+        intros lplayer cmt rplayer treeComp
+        cases lplayer with
+        | node _ _ _ =>
+          simp [treeCompArbGame] at treeComp
+        | leaf p =>
+          cases p with
+          | none => simp [treeCompArbGame] at treeComp
+          | some p =>
+            cases rplayer with
+            | node _ _ _ =>
+            simp [simultaneous_game]
+            | leaf _ =>
+                simp [treeCompArbGame] at treeComp
+                simp [simultaneous_game]
+                apply And.intro; exact treeComp.1;symm;exact treeComp.2
+      | node _ gl gr HIndL HIndR =>
+        intros lplayer cmt rplayer treeComp
+        cases lplayer with
+        | leaf _ => simp [treeCompArbGame] at treeComp
+        | node mprop lpl lpr =>
+          cases mprop with
+          | none =>  simp [treeCompArbGame] at treeComp
+          | some prop =>
+            cases rplayer with
+            | leaf _ => simp [simultaneous_game]
+            | node rp rpl rpr =>
+              match rp with
+              | none =>  simp [simultaneous_game]
+              | some rpv =>
+              simp [simultaneous_game]
+              simp [treeCompArbGame, gen_to_chooser] at treeComp
+              split
+              case isTrue eq => subst_eqs; simp at *; assumption
+              case isFalse neq =>
+                split
+                case isTrue eq1 =>
+                 subst_eqs; simp at *
+                 apply HIndR
+                 have comp : some (if rpv = prop then ChooserPrimMoves.Now else if rpv.1 = prop.1 then ChooserPrimMoves.Continue Chooser.Side.Right else ChooserPrimMoves.Continue Chooser.Side.Left) = ChooserPrimMoves.Continue Chooser.Side.Right
+                   := by {
+                   clear HIndR HIndL; simp; rw [ite_eq_iff]
+                   right
+                   apply And.intro
+                   · intro pp; apply neq; rw [pp]
+                   · rw [eq1]; simp
+                   }
+                 rw [comp] at treeComp ; simp at treeComp
+                 assumption
+                case isFalse neq2 =>
+                 apply HIndL
+                 have comp :some (if rpv = prop then ChooserPrimMoves.Now else if rpv.1 = prop.1 then ChooserPrimMoves.Continue Chooser.Side.Right else ChooserPrimMoves.Continue Chooser.Side.Left) = ChooserPrimMoves.Continue Chooser.Side.Left
+                   := by {
+                     simp; rw [ite_eq_iff]
+                     right
+                     apply And.intro
+                     · intro pp; apply neq; rw [pp]
+                     · simp; intro pp; apply neq2; rw [pp]
+                   }
+                 rw [comp] at treeComp; simp at treeComp
+                 simp
+                 assumption
+    · revert rplayer lplayer_commit lplayer
+      induction pub with
+      | leaf b =>
+        intros lplayer cmt rplayer simG
+        cases lplayer with
+        | node _ _ _ => simp [simultaneous_game] at simG
+        | leaf mp =>
+         cases mp with
+         | none =>
+           unfold simultaneous_game at simG
+           cases rplayer
+           all_goals { simp at simG }
+         | some p =>
+           simp [simultaneous_game] at simG
+           simp [treeCompArbGame]
+           apply And.intro
+           · exact simG.1
+           · symm; exact simG.2
+      | node _ gl gr HIndL HIndR =>
+        intros lplayer cmt rplayer simG
+        cases lplayer with
+        | leaf _ => simp [simultaneous_game] at simG
+        | node mp lpl lpr =>
+          cases mp with
+          | none =>
+            unfold simultaneous_game at simG;simp at simG
+            cases rplayer
+            all_goals { simp at simG }
+          | some p =>
+            cases rplayer with
+            | leaf _ => simp [treeCompArbGame]
+            | node mrp rpl rpr =>
+              cases mrp with
+              | none => simp [treeCompArbGame, gen_to_chooser]
+              | some rp =>
+              simp [simultaneous_game] at simG
+              simp [treeCompArbGame, gen_to_chooser]
+              split
+              case h_1 x heq =>
+                simp; injections; rename_i val_eq
+                rw [ite_eq_iff] at val_eq; simp at val_eq
+                cases val_eq with
+                | inl eq =>
+                  subst_eqs; simp at simG; assumption
+                | inr rest =>
+                  have nonsense := rest.2
+                  rw [ite_eq_iff] at nonsense
+                  simp at nonsense
+              case h_2 x heq =>
+                simp at heq
+                rw [ite_eq_iff] at heq
+                cases heq with
+                | inl ff => simp at ff
+                | inr hyp =>
+                  simp at HIndL
+                  apply HIndL
+                  -- have cf : (p = rp) = False := sorry
+                  rw [ite_cond_eq_false] at simG
+                  have ⟨ neq , neq1 ⟩ := hyp
+                  simp at neq1
+                  rw [ite_cond_eq_false] at simG
+                  assumption
+                  simp; intro pp; apply neq1; rw [pp]
+                  simp; intro pp; apply hyp.1; rw [pp]
 
 -- Elemen In Tree
 def simultaneous_elemenin_game {α ℍ : Type}
@@ -118,3 +250,32 @@ def simultaneous_elemenin_game {α ℍ : Type}
      | .leaf _ ,  _ , .node _ _ _ => .Left
      | .node _ _ _, .leaf _ , _ => .Right
      | .node _ _ _,  _ , .leaf _ => .Left
+
+-- * Data Rev
+-- def simultaneous_data_rev_game {α ℍ : Type}
+--   [o : Hash α ℍ][mag : HashMagma ℍ]
+--   [DecidableEq ℍ] -- This is BEq ℍ and LawfulBEq
+--   (len : Nat)
+--   -- Player 1
+--   (lplayer : ABTree (Option α) (Option (ℍ × ℍ)))
+--   (lplayer_commit : ℍ)
+--   -- Player 2 -- not symmetric game.
+--   (rplayer : ABTree (Option α) (Option (ℍ × ℍ)))
+--   (rplayer_commit : ℍ)
+--   --
+--   (hneq : ¬ lplayer_commit = rplayer_commit)
+--   --
+--   : Option SimWinner :=
+--   match len with
+--   | .zero =>
+--     match lplayer , rplayer with
+--     | .leaf lv ,.leaf lr => sorry
+--     | .leaf _ , _ => .some .Left
+--     | _ , .leaf _ => .some .Right
+--     | _ , _ => .none
+--   | .succ plen with
+--     match lplayer , rplayer with
+--     | .node ln ll lr, .node rn rl rr => sorry
+--     | .leaf _ , .node _ _ _ => .some .Rigth
+--     | .node _ _ _ , .leaf _ => .some .Left
+--     | _ , _ => .none
